rocq-osiris/theories/semantics/step.v
@@ -248,7 +248,8 @@ Definition phys_eq_val_store v1 v2 σ : option bool :=
   | VLoc l1, VLoc l2 =>
       Some (locations.eqb l1 l2)
   | VArray l1, VArray l2
-  | VRecord l1, VRecord l2 =>
+  | VRecord l1, VRecord l2
+  | VInline _ l1, VInline _ l2 =>
       match σ !! l1, σ !! l2 with
       | Some (Block Mut _), Some (Block _ _)
       | Some (Block _ _), Some (Block Mut _) => Some (locations.eqb l1 l2)
