rocq-osiris/theories/program_logic/rules/inline_rules.v
@@ -1,0 +1,77 @@
+From iris Require Import gen_heap proofmode.proofmode.
+From iris.bi.lib Require Import fractional.
+From osiris Require Import lang type_nel.
+Require Import osiris_utils.
+Require Import ewp.
+Require Import impure_rules stop_rules.
+Require Export record_rules.
+From osiris.utils Require Import list_z big_opLZ.
+
+(** This file defines record resource predicates and [imp] rules for inline-records. *)
+
+Section inline_record_reasoning.
+
+  Context `{!osirisGS Σ}.
+
+  Context {η : env} {E : coPset} {Ψ : iEff Σ}.
+
+  Local Instance notval_listval : NotVal (list val) := {}.
+
+  Local Instance encode_record c : Encode record := { encode' r := VInline c r }.
+
+  Lemma imp_EInline {τ : types} {ζ} (Φs : τ -#> iProp Σ) c t es :
+    let encode_rec := encode_record c in
+    τ_length τ ≤ max_array_length →
+    impure E (evals η es) Ψ ζ Φs -∗
+    impure E (eval η (EInline c t es)) Ψ ζ
+      (λ r, ∃# (xs : τ), ownBlock r 1 t xs ∗ Φs xs).
+  Proof.
+    iIntros (?) "%Hlength Hes". simpl_eval.
+    iApply (imp_bind with "Hes").
+    iIntros (xs) "HΦs".
+    iApply imp_bind.
+    { simpl.
+      replace (to_vals xs) with
+      (@observe (list val) (list val) (@observe_list val Encode_val) (to_vals xs)).
+      iApply (@imp_allocn _ _ _ _ _ val Encode_val (λ ls, [∗ listZ] l;v ∈ ls; (to_vals xs), l ↦ v)%I (to_vals xs)).
+      iIntros "!>" (ls) "$".
+      simpl. rewrite map_id. reflexivity. }
+    iIntros (ls) "Hls".
+    iPoseProof (big_sepLZ2_length with "Hls") as "%Hlength_ls".
+    iApply imp_bind.
+    { iApply imp_alloc_block.
+      iPureIntro. simpl.
+      rewrite Hlength_ls. rewrite to_vals_length. assumption. }
+    iIntros (r) "(Hmut & Hblocks)".
+    iApply imp_ret. encode.
+    rewrite bi_texist_equiv. iFrame.
+  Qed.
+
+End inline_record_reasoning.
+
+(* The [RecordRepr]/[ownRecord] machinery from [record_rules] applies to
+   inline records as well; we restate the construction rule in terms of a
+   user-provided logical model. *)
+
+Section encoded_fields.
+
+  Context `{!osirisGS Σ}.
+
+  Lemma imp_inline_record `{RecordRepr A τ t} {η E Ψ ζ} c es (Φs : τ -#> iProp Σ) :
+    let encode_rec := encode_record c in
+    (τ_length τ ≤ max_array_length)%Z →
+    impure E (evals η es) Ψ ζ Φs -∗
+    impure E (eval η (EInline c t es)) Ψ ζ (λ r, ∃# (xs : τ), ownRecord r 1 (types_to_repr xs) ∗ Φs xs).
+  Proof.
+    iIntros (? Hlength) "Hes".
+    iApply (imp_wand with "[-]").
+    { iApply (imp_EInline with "Hes"). assumption. }
+    iIntros (r).
+    rewrite !bi_texist_equiv.
+    iIntros "(%xs & Hr & HΦ)".
+    iFrame. unfold ownRecord.
+    pose proof repr_id as Hid. simpl in Hid. rewrite Hid.
+    iApply "Hr".
+  Qed.
+
+End encoded_fields.
